src/tls/StreamAE.fsti
@@ -81,7 +81,7 @@ let ctr (#l:rid) (#r:rid) (#i:id) (#log:log_ref l i) (c:seqn_ref r i log)
 		   else seqn i) 
 		increases) = c
 
-// TODO: make this abstract (currently impossible because of TestClient13.fst
+// kept concrete for log and counter, but the key and iv should be private.
 type state (i:id) (rw:rw) = 
   | State: #region:rid 
          -> #log_region:rid{if rw=Writer then region = log_region else HyperHeap.disjoint region log_region }
@@ -99,24 +99,39 @@ type state (i:id) (rw:rw) =
 type writer i = s:state i Writer
 type reader i = s:state i Reader
 
-//16-04-25 multiple-reader style: we fork new readers from the writer.
+// We generate first the writer, then the reader (possibly several of them)
 
-// Generate a fresh instance with index i in a fresh sub-region of r0
-// (we might drop this spec, since F* will infer something at least as precise,
-// but we keep it for documentation)
-val gen: parent:rid -> i:id -> ST (writer i)
-  (requires (fun h0 -> True))
-  (ensures  (fun h0 (w:writer i) h1 ->
+let genPost (#i:id) parent h0 (w:writer i) h1 = 
                modifies Set.empty h0 h1 /\
-               extends (w.region) parent /\
+               extends w.region parent /\
                fresh_region w.region h0 h1 /\
 	       (authId i ==>
   		      (m_contains (ilog w.log) h1 /\
 		       m_sel h1 (ilog w.log) = createEmpty)) /\
 	       m_contains (ctr w.counter) h1 /\
-	       m_sel h1 (ctr w.counter) == 0))
+	       m_sel h1 (ctr w.counter) == 0
+//16-04-30 how to share the whole ST ... instead of genPost?
 
-val genReader: parent:rid -> i:id -> w:writer i -> ST (reader i)
+// Generate a fresh instance with index i in a fresh sub-region of r0
+// (we might drop this spec, since F* will infer something at least as precise,
+// but we keep it for documentation)
+
+val gen: parent:rid -> i:id -> ST (writer i)
+  (requires (fun h0 -> True))
+  (ensures (genPost parent))
+
+
+// Coerce a writer with index i in a fresh subregion of parent
+// (coerced readers can then be obtained by calling genReader)
+val coerce: parent:rid -> i:id{~(authId i)} -> kv:key i -> iv:iv i -> ST (writer i)
+  (requires (fun h0 -> True))
+  (ensures  (genPost parent))
+
+val leak: #i:id{~(authId i)} -> role:rw -> state i role -> ST (key i * iv i)
+  (requires (fun h0 -> True))
+  (ensures  (fun h0 r h1 -> modifies Set.empty h0 h1 ))
+
+val genReader: parent:rid -> #i:id -> w:writer i -> ST (reader i)
   (requires (fun h0 -> HyperHeap.disjoint parent w.region)) //16-04-25  we may need w.region's parent instead
   (ensures  (fun h0 (r:reader i) h1 ->
                modifies Set.empty h0 h1 /\
@@ -129,30 +144,27 @@ val genReader: parent:rid -> i:id -> w:writer i -> ST (reader i)
 // encryption (on concrete bytes), returns (cipher @| tag)
 // Keeps seqn and nonce implicit; requires the counter not to overflow
 // encryption of plaintexts; safe instances are idealized
-val encrypt:
-  i:id -> e:writer i -> l:plainLen -> p:plain i l -> ST (cipher i l)
+
+val encrypt: #i:id -> e:writer i -> l:plainLen -> p:plain i l -> ST (cipher i l)
     (requires (fun h0 -> 
     	  is_seqn i (m_sel h0 (ctr e.counter) + 1)))
     (ensures  (fun h0 c h1 ->
-                           modifies (Set.singleton e.region) h0 h1
-                         /\ (authId i ==> m_contains (ilog e.log) h1)
-                         /\ m_contains (ctr e.counter) h1
-                         /\ m_sel h1 (ctr e.counter) == m_sel h0 (ctr e.counter) + 1
-			 /\ authId i ==> 
+                 modifies (Set.singleton e.region) h0 h1 /\
+                 (authId i ==> m_contains (ilog e.log) h1) /\
+                 m_contains (ctr e.counter) h1 /\
+                 m_sel h1 (ctr e.counter) == m_sel h0 (ctr e.counter) + 1 /\
+	         authId i ==> 
 			    (let log = ilog e.log in
  			     let ent = Entry l c p in
 			     let n = Seq.length (m_sel h0 log) in
-			      m_contains log h1
-   			   /\ witnessed (MonotoneSeq.at_least n ent log)
-                           /\ m_sel h1 log = snoc (m_sel h0 log) ent)))
+			      m_contains log h1 /\
+   			      witnessed (MonotoneSeq.at_least n ent log) /\
+                              m_sel h1 log = snoc (m_sel h0 log) ent)))
 
-let matches #i l (c: cipher i l) (Entry l' c' _) =
-  l = l' && c = c'
+let matches #i l (c: cipher i l) (Entry l' c' _) = l = l' && c = c'
 
 // decryption, idealized as a lookup of (c,ad) in the log for safe instances
-val decrypt:
-  i:id -> d:reader i -> l:plainLen -> c:cipher i l
-  -> ST (option (plain i l))
+val decrypt: #i:id -> d:reader i -> l:plainLen -> c:cipher i l -> ST (option (plain i l))
   (requires (fun h0 -> is_seqn i (m_sel h0 (ctr d.counter) + 1)))
   (ensures  (fun h0 res h1 ->
 	      (authId i ==>
